src/WeakestAdequacy.v
@@ -1,35 +1,131 @@
 Unset Universe Checking.
 From sflib Require Import sflib.
 From Paco Require Import paco.
-From Fairness Require Import ITreeLib IProp IPM ModSim ModSimNat PCM Weakest Concurrency.
+From Fairness Require Import ITreeLib IProp IPM ModSim ModSimNat PCM Weakest Concurrency ModAdequacy.
 Require Import Program.
 
 Set Implicit Arguments.
 
+
 Module WSim.
   Section WSIM.
-    Context `{Σ: GRA.t}.
-
     Variable md_src: Mod.t.
     Variable md_tgt: Mod.t.
 
 
+    Context `{Σ: GRA.t}.
+    Context `{MONORA: @GRA.inG monoRA Σ}.
+    Context `{THDRA: @GRA.inG ThreadRA Σ}.
+    Context `{STATESRC: @GRA.inG (stateSrcRA md_src.(Mod.state)) Σ}.
+    Context `{STATETGT: @GRA.inG (stateTgtRA md_tgt.(Mod.state)) Σ}.
+    Context `{IDENTSRC: @GRA.inG (identSrcRA md_src.(Mod.ident)) Σ}.
+    Context `{IDENTTGT: @GRA.inG (identTgtRA md_tgt.(Mod.ident)) Σ}.
+    Context `{OBLGRA: @GRA.inG ObligationRA.t Σ}.
+    Context `{ARROWRA: @GRA.inG (ArrowRA md_tgt.(Mod.ident)) Σ}.
+    Context `{EDGERA: @GRA.inG EdgeRA Σ}.
+    Context `{ONESHOTRA: @GRA.inG (@FiniteMap.t (OneShot.t unit)) Σ}.
+    Variable init_res: Σ.
+    Hypothesis RESWF: URA.wf (init_res ⋅ (@default_initial_res _ md_src.(Mod.state) md_tgt.(Mod.state) md_src.(Mod.ident) md_tgt.(Mod.ident) _ _ _ _ _ _ _)).
 
-(*     list_prop_sum (fun '(tid, f_src, f_tgt) => *)
+    Definition initial_prop (ths: TIdSet.t) o: iProp :=
+      ((FairRA.whites (fun _ => True: Prop) o)
+         **
+         (FairRA.blacks (fun i => match i with | inr _ => True | _ => False end: Prop))
+         **
+         (natmap_prop_sum ths (fun tid _ => ObligationRA.duty (inl tid) []))
+         **
+         (natmap_prop_sum ths (fun tid _ => own_thread tid))
+         **
+         (St_src md_src.(Mod.st_init))
+         **
+         (St_tgt md_tgt.(Mod.st_init)))%I
+    .
 
-(* (p_src, p_tgt) *)
 
-(*     Record sim (p_src: Th.t _) (p_tgt: Th.t _) : Prop := *)
-(*       mk { *)
-(*           funs: forall im_tgt, *)
-(*           exists im_src rs r_shared I, *)
-(*             (<<INIT: I (key_set p_src, im_src, im_tgt, md_src.(Mod.st_init), md_tgt.(Mod.st_init)) r_shared>>) /\ *)
-(*               (<<SIM: Forall3 *)
-(*                         (fun '(t1, src) '(t2, tgt) '(t3, r) => *)
-(*                            (t1 = t2 /\ t1 = t3) /\ *)
-(*                            @local_sim_init _ md_src.(Mod.state) md_tgt.(Mod.state) md_src.(Mod.ident) md_tgt.(Mod.ident) wf_src wf_tgt I _ _ (@eq Any.t) r t1 src tgt) *)
-(*                         (Th.elements p_src) (Th.elements p_tgt) (NatMap.elements rs)>>) /\ *)
-(*               (<<WF: URA.wf (r_shared ⋅ NatMap.fold (fun _ r s => r ⋅ s) rs ε)>>) *)
-(*         }. *)
-  End MODSIM.
-End UserSim.
+    Section WHOLE_PROGRAM_SIM.
+      Variable c: list (fname * Any.t).
+
+      Definition fun_pairs :=
+        (NatMapP.of_list (numbering (List.map (fun '(fn, arg) => (fn2th md_src fn arg, fn2th md_tgt fn arg)) c))).
+
+      Record whole_sim: Prop :=
+        mk_whole_sim {
+            I_whole: list iProp;
+            init_whole:
+            exists o,
+              ((initial_prop (NatMapP.of_list (numbering (List.map (fun _ => tt) c))) o) (* INIT *)
+                 -∗
+                 (#=>
+                    ((mset_all (nth_default True%I I_whole) (topset I_whole)) (* I *)
+                       **
+                       (natmap_prop_sum
+                          fun_pairs
+                          (fun tid '(th_src, th_tgt) =>
+                             stsim
+                               I_whole tid (topset I_whole)
+                               ibot5 ibot5
+                               (fun r_src r_tgt => own_thread tid ** ObligationRA.duty (inl tid) [] ** ⌜r_src = r_tgt⌝)
+                               th_src th_tgt)))))
+          }.
+
+      Lemma whole_sim_implies_usersim
+            (SIM: whole_sim)
+        :
+        UserSim.sim md_src md_tgt (prog2ths md_src c) (prog2ths md_tgt c).
+      Proof.
+        (* just a casting *)
+      Admitted.
+
+      Lemma whole_sim_implies_refinement
+            (SIM: whole_sim)
+        :
+        Adequacy.improves (interp_all md_src.(Mod.st_init) (prog2ths md_src c) 0)
+                          (interp_all md_tgt.(Mod.st_init) (prog2ths md_tgt c) 0).
+      Proof.
+        eapply usersim_adequacy. eapply whole_sim_implies_usersim. auto.
+      Qed.
+    End WHOLE_PROGRAM_SIM.
+
+
+    Section CONTEXT_SIM.
+      Record context_sim: Prop :=
+        mk_context_sim {
+            I_ctx: list iProp;
+            init_ctx:
+            exists o,
+              ((initial_prop TIdSet.empty o) (* INIT *)
+                 -∗
+                 (#=> (mset_all (nth_default True%I I_ctx) (topset I_ctx))));
+            funs_ctx:
+            forall tid fn arg,
+              (own_thread tid)
+                -∗
+                (ObligationRA.duty (inl tid) [])
+                -∗
+                (stsim
+                   I_ctx tid (topset I_ctx)
+                   ibot5 ibot5
+                   (fun r_src r_tgt => own_thread tid ** ObligationRA.duty (inl tid) [] ** ⌜r_src = r_tgt⌝)
+                   (fn2th md_src fn arg) (fn2th md_tgt fn arg))
+          }.
+
+      Lemma context_sim_implies_modsim
+            (SIM: context_sim)
+        :
+        ModSim.mod_sim md_src md_tgt.
+      Proof.
+        (* just a casting *)
+      Admitted.
+
+      Lemma context_sim_implies_contextual_refinement
+            (SIM: context_sim)
+        :
+        forall p,
+          Adequacy.improves (interp_all md_src.(Mod.st_init) (prog2ths md_src p) 0)
+                            (interp_all md_tgt.(Mod.st_init) (prog2ths md_tgt p) 0).
+      Proof.
+        eapply modsim_adequacy. eapply context_sim_implies_modsim. auto.
+      Qed.
+    End CONTEXT_SIM.
+  End WSIM.
+End WSim.
